

$$a) T(z) = 1 + z^{-1} + z^{-2} + z^{-3} = z^3 + z^2 + z + 1$$

$$T(z) = e^{j\omega}$$

$$H(\omega) = \frac{1}{e^0} + e^{j\omega} + e^{j\omega^2} + e^{3j\omega}$$

$$= e^{j1.5\omega} (e^{j1.5\omega} + e^{j0.5\omega} + e^{-j0.5\omega} + e^{-1.5j\omega})$$

$$\angle H(\omega) = 1.5\omega$$

$$|H(\omega)| = \underbrace{|e^{j1.5\omega}|}_{1} |e^{j\omega \cdot 1.5} + e^{j \cdot 0.5\omega} + e^{-j0.5\omega} + e^{-1.5j\omega}|$$

$$(e^{j1.5\omega} + e^{-1.5j\omega}) + (e^{j0.5\omega} + e^{-j0.5\omega})$$

$$= 2\cos(1.5\omega) + 2\cos(0.5\omega)$$

$$\Rightarrow |H(\omega)| = 2 \cdot |\cos(1.5\omega) + \cos(0.5\omega)|$$



$$b) z^4 + z^3 + z^2 + z + 1$$

$$= e^{4j\omega} + e^{3j\omega} + e^{2j\omega} + e^{j\omega} + e^0 = e^{2j\omega} (e^{2j\omega} + e^{j\omega} + 1 + e^{-j\omega} + e^{-2j\omega})$$

$$\Rightarrow \angle H(\omega) = 2\omega$$

$$\Rightarrow |H(\omega)| = \underbrace{|e^{2j\omega}|}_1 \underbrace{|e^{2j\omega} + e^{-2j\omega} + e^{j\omega} + e^{-j\omega} + 1|}_{|2\cos(2j\omega) + 2\cos(j\omega) + 1|}$$

c)  $T(z) = z - 1$  → normalizada

$T(\omega)$  es  $T(z)$  con  $z = e^{j\omega}$

$$|T(\omega)| = |e^{j\omega} - 1| = \underbrace{|e^{0.5j\omega}|}_{=1} \cdot |e^{0.5j\omega} - e^{-0.5j\omega}|$$

$$= |\cos(0.5\omega) + j \cdot \sin(0.5\omega) - [\cos(0.5\omega) - j \cdot \sin(0.5\omega)]|$$

$$= |2j \sin(0.5\omega)|$$

$$\Rightarrow |T(\omega)| = 2 \cdot |\sin(0.5\omega)|$$

$$\Rightarrow \angle T(z) = 0.5\omega$$



$$d) T(z) = z^2 - 1$$

$$H(\omega) = e^{zj\omega} - e^0 = e^{j\omega} (e^{j\omega} + e^{-j\omega})$$

$$\Rightarrow \angle H(\omega) = \omega \quad \Rightarrow |H(\omega)| = \underbrace{|e^{j\omega}|}_1 |e^{j\omega} + e^{-j\omega}|$$
$$|2\cos(j\omega)|$$